theories/factorial/factorial.v
@@ -5,13 +5,16 @@ Require Import String.
 Require Import ZArith.
 Require Import List.
 Require Import Bool.
+Require Import ExtrOcamlBasic.
+Require Import ExtrOcamlString.
+Extraction Language OCaml.
 Open Scope string_scope.
 Open Scope Z_scope.
 Open Scope volpic_notation.
 Import ListNotations.
 
 
-Definition factorial (VP_store: store) := 
+Definition factorial (VP_store: store) (VP_loop_limit: nat) := 
 	let VP_poison := false in
 	let (VP_store,VP_poison) := 
 		(if (negb VP_poison) then
@@ -20,42 +23,171 @@ Definition factorial (VP_store: store) :=
  			(VP_store,true)) in
 	let (VP_store,VP_poison) := 
 		(if (negb VP_poison) then
- 			 (while ( fun VP_store => 1 <=? get_int VP_store "VP_X" ) with VP_store upto 1000%nat begin fun VP_store => (*Block: next 2 statements*)
-		let VP_store := update VP_store "VP_result" (VInteger ( get_int VP_store "VP_result" * get_int VP_store "VP_X" )) in
-update VP_store "VP_X" (VInteger ( get_int VP_store "VP_X" - 1 )) end,VP_poison) 
+ 			 (match 
+(while ( fun VP_store => 1 <=? get_int VP_store "VP_X" ) with VP_store upto VP_loop_limit begin fun VP_store => (*Block: next 2 statements*)
+			let VP_store := update VP_store "VP_result" (VInteger ( get_int VP_store "VP_result" * get_int VP_store "VP_X" )) in
+update VP_store "VP_X" (VInteger ( get_int VP_store "VP_X" - 1 )) end) with 
+ 		 | None => (VP_store,true)
+		 | Some VP_store' => (VP_store',VP_poison)
+		 	 end) 
 		else
  			(VP_store,true)) in
-VP_store.
+(VP_store,VP_poison).
+Extraction "factorial.ml" factorial.
 
-Definition main (VP_store: store) := 
-	let VP_poison := false in
-	let (VP_store,VP_poison) := 
-		(if (negb VP_poison) then
- 			 ((*Block: next 6 statements*)
-(*	let VP_store := fpc_write_text_shortstr VP_store ("n: ") 0 in*)
-(*	let VP_store := fpc_write_end VP_store in*),VP_poison) 
-		else
- 			(VP_store,true)) in
-	let (VP_store,VP_poison) := 
-		(if (negb VP_poison) then
- 			 ((*Block: next 6 statements*)
-(*	let VP_store := fpc_read_text_shortstr VP_store 255 (get_string VP_store "VP_I") in*)
-(*	let VP_store := fpc_readln_end VP_store in*),VP_poison) 
-		else
- 			(VP_store,true)) in
-	let (VP_store,VP_poison) := 
-		(if (negb VP_poison) then
- 			 (update VP_store "VP_N" (VInteger ( get_int (StrToInt VP_store (get_string VP_store "VP_I")) "VP_result" )),VP_poison) 
-		else
- 			(VP_store,true)) in
-	let (VP_store,VP_poison) := 
-		(if (negb VP_poison) then
- 			 ((*Block: next 7 statements*)
-(*	let VP_store := fpc_write_text_shortstr VP_store ("fact(n): ") 0 in*)
-(*	let VP_store := fpc_write_text_sint VP_store (get_int (factorial VP_store (get_int VP_store "VP_N")) "VP_result") 0 in*)
-(*	let VP_store := fpc_writeln_end VP_store in*),VP_poison) 
-		else
- 			(VP_store,true)) in
-VP_store.
+(*Ignored $main*)
 
-Compute (main fresh_store).
+(* Proof ensues *)
+
+Require Import FunctionalExtensionality.
+
+Lemma update_shadow : forall (m : store) x v1 v2,
+  (x !-> v2 ; x !-> v1 ; m) = (x !-> v2 ; m).
+Proof.
+  intros. apply functional_extensionality. intros.
+  unfold update. destruct (String.eqb x0 x) eqn:E; reflexivity.
+Qed.
+
+Lemma update_eq : forall (m : store) x v,
+	(x !-> v; m) x = v.
+Proof.
+	intros. unfold update. now rewrite String.eqb_refl.
+Qed.
+
+Lemma update_neq : forall (m : store) x y v,
+	x <> y ->
+	(x !-> v; m) y = m y.
+Proof.
+	intros. unfold update. destruct (eqb_neq x y). now rewrite String.eqb_sym, (H1 H).
+Qed.
+
+Theorem update_permute : 
+  forall (m : store)
+    v1 v2 x1 x2,
+  x2 <> x1 ->
+  (x1 !-> v1 ; x2 !-> v2 ; m)
+  =
+  (x2 !-> v2 ; x1 !-> v1 ; m).
+Proof.
+  intros. apply functional_extensionality. intros.
+  unfold update. destruct (x =? x1)%string eqn:E, (x =? x2)%string eqn:E'; auto.
+  pose (String.eqb_eq x x1). pose (String.eqb_eq x x2).
+  destruct i, i0. specialize (H0 E). specialize (H2 E'). subst. contradiction.
+Qed.
+
+Definition Z_fact (n : Z) := Z.of_nat (fact (Z.to_nat n)).
+
+Lemma fact_sub : forall n,
+	(1 <= n)%nat ->
+	fact n = (n * fact (n - 1))%nat.
+Proof.
+	induction n; intros; simpl in *.
+	inversion H. now rewrite Nat.sub_0_r.
+Qed.
+
+Require Import Lia.
+
+Lemma Z_fact_sub : forall n,
+	1 <= n ->
+	Z_fact n = n * Z_fact (n - 1).
+Proof.
+	intros. replace n with (Z.of_nat (Z.to_nat n)).
+	unfold Z_fact. rewrite Nat2Z.id. 
+		replace (Z.of_nat (Z.to_nat n) - 1) with (Z.of_nat (Z.to_nat (n - 1))). 
+		rewrite Nat2Z.id. 
+		rewrite <- Nat2Z.inj_mul, Z2Nat.inj_sub. replace (Z.to_nat 1) with 1%nat. 
+		rewrite fact_sub; lia. all: lia.
+Qed.
+
+Lemma nle_1_destruct : forall n,
+	~ (1 <= n) ->
+	n = 0 \/ exists p, n = Z.neg p.
+Proof.
+	intros.	destruct n; try lia.
+	right. now exists p.
+Qed.
+
+Lemma Z_fact_nle_1 : forall n,
+	(1 <=? n) = false ->
+	Z_fact n = 1.
+Proof.
+	intros. apply Z.leb_nle in H. apply nle_1_destruct in H. destruct H; subst.
+	reflexivity. destruct H. subst. reflexivity.
+Qed.
+
+Definition output_safe (f : store -> nat -> store * bool) 
+		input expected :=
+	forall loop_limit output
+	  (Terminates: (output, false) = f input loop_limit),
+	  output "VP_result" = expected.
+
+Ltac vpex :=
+	match goal with [H: (?fst, ?snd) = 
+		match ?m with (Some s) => ?s' | None => ?n' end |- _] =>
+			let name := fresh "body" in
+			remember m as name
+		| [H: (?fst, ?snd) = (let (st, ps) := 
+			match ?m with (Some s) => ?s' | None => ?n' end in _) |- _] =>
+			let E := fresh "Eq" in 
+			destruct m eqn:E
+	end || idtac "No match".
+
+Theorem factorial_correct : forall n st,
+	output_safe factorial ("VP_X" !-> VInteger n; st) (VInteger (Z_fact n)).
+Proof.
+	unfold output_safe. intros. 
+	(* 
+		When dealing with fixpoints, we almost always want to induct over their
+		decreasing argument, because this will "turn the crank" and evaluate another
+		iteration of the loop.
+
+		There's an issue though: if we induct too early over
+		the decreasing argument (loop_limit in VOLPIC-lifted code), we end up with
+		an inductive hypothesis that refers to code outside of the fixpoint. This is
+		no good, because it generally ends up over-specializing our assumptions,
+		making them unusable.
+
+		The solution is to simplify until we get to just the loop in our termination
+		hypothesis. Note: this technique will need more refinement if there is code
+		after the loop.
+	*)
+	unfold factorial in Terminates. simpl in Terminates.
+	(*
+		We end up with a termination hypothesis that looks like
+			(output, false) := (let (VP_store, VP_poison) := <code> in (VP_store, VP_poison)).
+
+		This is annoying, because we can't use `inversion` or `simpl` to do any 
+		of the substitution that would seem intuitive at this point.
+
+		The `vpex` tactic looks for patterns like these and destructs the <code> terms,
+		unfolding the `let _ := _ in _` notation, making it much easier to 
+		write sub-proofs about them.
+	*)
+	vpex; inversion Terminates. subst. clear Terminates.
+	(*
+		We will often need some clever generalizations in proofs such as these.
+		These loosely resemble loop invariants that we'd have to write if we were
+		dealing with the same code in an imperative model using Hoare logic.
+	*)
+	replace (Z_fact n) with (1 * Z_fact n) by lia. 
+		generalize dependent n. generalize 1 at 3 4 as inter_prod.
+	(* 
+		Finally - we can do our induction. We will always get a trivial case where
+		the loop limit is zero, causing an early termination, which poisons the store.
+	*)
+	induction loop_limit; intros. inversion Eq.
+	match goal with [H: forall i n, ?x ?l ?b ?store = _ -> _ |- _] => 
+		remember x as loop_body end.
+	(* We can now start to reduce some of the assignments that have built up *) 
+	unfold get_int in Eq.
+	rewrite update_neq, update_eq, update_eq, update_neq, update_neq, update_eq in Eq;
+		try discriminate.
+	(* We have a conditional value for our output store, so let's do a case analysis *)
+	destruct (1 <=? n) eqn:E.
+	- rewrite update_shadow, update_permute, update_shadow in Eq; try discriminate.
+		(* Now we see why we generalized before inducting *)
+		erewrite IHloop_limit. rewrite <- Z.mul_assoc, <- Z_fact_sub.
+			reflexivity. lia. assumption.
+	- inversion Eq; subst. rewrite update_eq.
+		now rewrite Z_fact_nle_1, Z.mul_1_r.
+Qed.
